proof/extraction/Generic.ec
@@ -21,20 +21,6 @@ module Memcpy = {
     return out;
   }
 
-  proc _x_memcpy_u8u8p(out:W8.t list, in_ptr:W64.t) : W8.t list = {
-
-    var i:W64.t;
-
-    i <- (W64.of_int 0);
-
-    while ((i \ult (W64.of_int (size out)))) {
-      out <- put out (W64.to_uint i) (loadW8 Glob.mem (W64.to_uint (in_ptr + i)));
-      i <- (i + (W64.of_int 1));
-    }
-
-    return out;
-  }
-
   proc __memcpy_u8u8_2 (out:W8.t list, in_0:W8.t list, in_offset:W64.t,
                           bytes:W64.t) : W8.t list * W64.t = {
 
@@ -53,55 +39,81 @@ module Memcpy = {
 
 module BaseWGeneric = {
   proc __base_w (output : W32.t list, input : W8.t list) : W32.t list = {
-
+    
     var in_0:W64.t;
-    var out:W64.t;
     var bits:W64.t;
-    var consumed:W64.t;
-    var total:W8.t;
-    var total_32:W32.t;
+    var total:W32.t;
+    var i:W64.t;
     var _of_:bool;
     var _cf_:bool;
     var _sf_:bool;
     var _zf_:bool;
     var  _0:bool;
-
-    in_0 <- W64.zero;
-    out <- W64.zero;
-    bits <- W64.zero;
-    consumed <-W64.zero;
-    total <- W8.zero;
-
-    while ((consumed \ult (W64.of_int (size output)))) {
-      if (bits = W64.zero) {
-        total <- nth witness input (W64.to_uint in_0);
+    
+    in_0 <- (W64.of_int 0);
+    bits <- (W64.of_int 0);
+    total <- (W32.of_int 0);
+    i <- (W64.of_int 0);
+    
+    while ((i \ult (W64.of_int (size output)))) {
+      if ((bits = (W64.of_int 0))) {
+        total <- (zeroextu32 (nth witness input (W64.to_uint in_0)));
         in_0 <- (in_0 + (W64.of_int 1));
         bits <- (bits + (W64.of_int 8));
-      }
+      } 
       
       bits <- (bits - (W64.of_int 4));
-      total_32 <- (zeroextu32 total);
-      (_of_, _cf_, _sf_,  _0, _zf_, total_32) <- SHR_32 total_32 (truncateu8 bits);
-      total_32 <- (total_32 `&` (W32.of_int (16 - 1)));
-      output <- put output (W64.to_uint out) total_32; (* output.[(W64.to_uint out)] <- total_32; *)
-      out <- (out + (W64.of_int 1));
-      consumed <- (consumed + (W64.of_int 1));
+      (_of_, _cf_, _sf_,  _0, _zf_, total) <- SHR_32 total (truncateu8 bits);
+      total <- (total `&` (W32.of_int (16 - 1)));
+      output <- put output (W64.to_uint i) total;
+      i <- (i + (W64.of_int 1));
     }
-
     return (output);
   }
 }.
 
 module Memset = {
-  proc memset_u8 (a:W8.t list, inlen : W64.t, value:W8.t) : W8.t list = {
+  proc memset_u8 (a : W8.t list, value : W8.t) : W8.t list = {
 
     var i:W64.t;
     i <- (W64.of_int 0);
     
-    while ((i \ult inlen)) {
+    while ((i \ult (W64.of_int (size a)))) {
       a <- put a (W64.to_uint i) value;
       i <- (i + (W64.of_int 1));
     }
+
     return (a);
   }
 }.
+
+lemma memset_post (s : W8.t list, v : W8.t) :
+    hoare [Memset.memset_u8 : size s <= 128 ==> (* all ((=) v) res *)
+    forall (k : int), 0 <= k < size s => nth witness res k = v].
+proof.
+proc.
+wp;
+while (#pre /\ 0 <= to_uint i <= to_uint (W64.of_int (size s)) /\ forall (k : int), 0 <= k < to_uint i => nth witness s (to_uint i) = v); auto => />.
+- auto => /> * ; do split.
+  + smt(@W64).
+  + move => ?. rewrite to_uintD_small of_uintK ; admit.
+  + admit.
+- move => ?. do split.
+  + smt(@W64).
+  + smt.
+  + auto => /> *. admit.
+qed.
+
+lemma memset_ll : phoare [ Memset.memset_u8 : 4 <= size a <= 128 ==> true ] = 1%r.
+proof.
+proc.
+sp.
+while (#pre /\ 0 <= to_uint i <= size a) ((size a) - (to_uint i)) ; auto => /> *.
+- do split. 
+  + admit.
+  + rewrite size_put. assumption.
+  + rewrite size_put. move => ?. assumption.
+  + rewrite size_put /#.
+  + rewrite size_put. admit.
+- split ; [apply size_ge0 | smt()].
+qed.
